[move-prover] Cleaning prelude and experimenting with vector theories.
This cleans up the prelude (in the boogie v2 backend), pulling out general data structures like vectors and multisets into independent files and making them generic using Boogie's new monomorphization feature. It also supports now multiple theories for vectors with and without extensionality using the new `--vector-theory` flag. However, only the style of theory we had until now (Boogie arrays wo/ extensional equality) works well in all scenarios.

The supported theories are:

- `--vector-theory=BoogieArray` (default): similar like old `$ValueArray` (now type `Vec $Value`).
- `--vector-theory=BoogieArrayIntern`: attempt to make vectors extensional by introducing an internalization function s.t. `$IsEqual(v1, v2) <==> $Intern(v1) == $Intern(v2)`. Works semantically but times out on simple examples like `simple_vector_client.move`.
- `--vector-theory=SmtSeq`: uses smt sequence types. Too slow and times out on basic examples in `simple_vector_client.move` test.
- `--vector-theory=SmtArray`: use native array theory instead of Boogie array theory. Behaves mostly similar regards timing than `BoogieArray` but times out for the framework in some cases.
- `--vector-theory=SmtArrayExt`: use native array theory and adds axioms for extensionality, as done also with Boogie `--lib` flag. Times out on simple examples.

There is also a new script `tools/benchmark.sh` for recording verification times of a given set of modules, and some of its results in `tools/data`.

Most relevant changes of this PR are still off by default and guarded by the `--vnext` flag.

Closes: #8056

language/move-prover/boogie-backend-v2/src/boogie_helpers.rs
@@ -16,6 +16,8 @@ use move_model::{
     ty::{PrimitiveType, Type},
 };
 
+pub const MAX_MAKE_VEC_ARGS: usize = 12;
+
 /// Return boogie name of given module.
 pub fn boogie_module_name(env: &ModuleEnv<'_>) -> String {
     let name = env.symbol_pool().string(env.get_name().name());
@@ -189,14 +191,22 @@ pub fn boogie_type_value_array(env: &GlobalEnv, args: &[Type]) -> String {
 
 /// Creates a type value array for types given as strings.
 pub fn boogie_type_value_array_from_strings(args: &[String]) -> String {
+    boogie_make_vec_from_strings(args)
+}
+
+/// Creates a vector from the given list of arguments.
+pub fn boogie_make_vec_from_strings(args: &[String]) -> String {
     if args.is_empty() {
-        return "$EmptyTypeValueArray".to_string();
+        "EmptyVec()".to_string()
+    } else {
+        let n = usize::min(args.len(), MAX_MAKE_VEC_ARGS);
+        let direct_args = &args[0..n];
+        let mut make = format!("MakeVec{}({})", n, direct_args.iter().join(", "));
+        for arg in args.iter().skip(n) {
+            make = format!("ExtendVec({}, {})", make, arg)
+        }
+        make
     }
-    let mut map = String::from("$MapConstTypeValue($DefaultTypeValue())");
-    for (i, arg) in args.iter().enumerate() {
-        map = format!("{}[{} := {}]", map, i, arg);
-    }
-    format!("$TypeValueArray({}, {})", map, args.len())
 }
 
 /// Return boogie type for a local with given signature token.
@@ -210,7 +220,7 @@ pub fn boogie_local_type(ty: &Type) -> String {
             TypeValue => "$TypeValue".to_string(),
             _ => panic!("unexpected type"),
         },
-        Vector(..) | Struct(..) => "$ValueArray".to_string(),
+        Vector(..) | Struct(..) => "Vec $Value".to_string(),
         Reference(..) => "$Mutation".to_string(),
         TypeParameter(..) => "$Value".to_string(),
         Fun(..) | Tuple(..) | TypeDomain(..) | ResourceDomain(..) | TypeLocal(..) | Error
@@ -220,7 +230,7 @@ pub fn boogie_local_type(ty: &Type) -> String {
 
 pub fn boogie_declare_temps() -> String {
     "var $$t_bool: bool;\nvar $$t_int: int;\nvar $$t_addr: int;\nvar $$t_type: $TypeValue;\
-    \nvar $$t, $$t1, $$t2, $$t3: $Value;\nvar $$t_vec: $ValueArray;"
+    \nvar $$t, $$t1, $$t2, $$t3: $Value;\nvar $$t_vec: Vec $Value;"
         .to_string()
 }
 
@@ -288,7 +298,7 @@ fn boogie_well_formed_expr_impl(env: &GlobalEnv, name: &str, ty: &Type, nest: us
             ));
             if !matches!(**elem_ty, Type::TypeParameter(..)) {
                 let suffix = boogie_type_suffix(elem_ty);
-                let nest_value = &format!("$ReadValueArray({},$${})", name, nest);
+                let nest_value = &format!("ReadVec({},$${})", name, nest);
                 let mut check = format!("$IsValidBox{}({})", suffix, nest_value);
                 let nest_value_unboxed = &format!("$Unbox{}({})", suffix, nest_value);
                 let nest_check = boogie_well_formed_expr_impl(
@@ -301,21 +311,21 @@ fn boogie_well_formed_expr_impl(env: &GlobalEnv, name: &str, ty: &Type, nest: us
                     check = format!("{} &&\n  {}", check, nest_check);
                 }
                 add_type_check(format!(
-                    "(forall $${}: int :: {{{}}}\n{}    $${} >= 0 && $${} < $LenValueArray({}) ==> {})",
-                    nest, nest_value, indent, nest, nest, name, check,
+                    "(forall $${}: int :: {{{}}}\n{}    $InRangeVec({}, $${}) ==> {})",
+                    nest, nest_value, indent, name, nest, check,
                 ));
             }
         }
         Type::Struct(module_idx, struct_idx, targs) => {
             let struct_env = env.get_module(*module_idx).into_struct(*struct_idx);
             add_type_check(format!(
-                "$Tag{}({}) && $ValueArray_$is_well_formed({})",
+                "$Tag{}({}) && $IsValidU64(LenVec({}))",
                 boogie_struct_name(&struct_env),
                 name,
                 name
             ));
             add_type_check(format!(
-                "$LenValueArray({}) == {}",
+                "LenVec({}) == {}",
                 name,
                 struct_env.get_field_count()
             ));
@@ -323,11 +333,7 @@ fn boogie_well_formed_expr_impl(env: &GlobalEnv, name: &str, ty: &Type, nest: us
             for field_env in struct_env.get_fields() {
                 let ty = field_env.get_type().instantiate(targs);
                 let suffix = boogie_type_suffix(&ty);
-                let field_value = format!(
-                    "$ReadValueArray({}, {})",
-                    name,
-                    boogie_field_name(&field_env)
-                );
+                let field_value = format!("ReadVec({}, {})", name, boogie_field_name(&field_env));
                 add_type_check(format!("$IsValidBox{}({})", suffix, field_value));
                 let nest_check = boogie_well_formed_expr_impl(
                     env,
@@ -431,23 +437,12 @@ pub fn boogie_global_declarator(
     }
 }
 
-pub fn boogie_byte_blob(options: &BoogieOptions, val: &[u8]) -> String {
-    if options.vector_using_sequences {
-        // Use concatenation.
-        let mut res = "$mk_vector()".to_string();
-        for b in val {
-            res = format!("$push_back_vector({}, $Integer({}))", res, b);
-        }
-        res
-    } else {
-        // Repeated push backs very expensive in map representation, so construct the value
-        // array directly.
-        let mut ctor_expr = "$MapConstValue($DefaultValue())".to_owned();
-        for (i, b) in val.iter().enumerate() {
-            ctor_expr = format!("{}[{} := $Integer({})]", ctor_expr, i, *b);
-        }
-        format!("$ValueArray({}, {})", ctor_expr, val.len())
-    }
+pub fn boogie_byte_blob(_options: &BoogieOptions, val: &[u8]) -> String {
+    let args = val
+        .iter()
+        .map(|v| format!("$Box_int({})", *v))
+        .collect_vec();
+    boogie_make_vec_from_strings(&args)
 }
 
 /// Construct a statement to debug track a local based on the Boogie attribute approach.
