language/move-prover/boogie-backend-v2/src/prelude/multiset-array-theory.bpl
@@ -1,0 +1,44 @@
+// Copyright (c) The Diem Core Contributors
+// SPDX-License-Identifier: Apache-2.0
+
+// Boogie model for multisets, based on Boogie arrays. This theory assumes extensional equality for element types.
+
+type {:datatype} Multiset _;
+function {:constructor} Multiset<T>(v: [T]int, l: int): Multiset T;
+
+function {:builtin "MapConst"} MapConstMultiset<T>(l: int): [T]int;
+
+function {:inline} EmptyMultiset<T>(): Multiset T {
+    Multiset(MapConstMultiset(0), 0)
+}
+
+function {:inline} LenMultiset<T>(s: Multiset T): int {
+    l#Multiset(s)
+}
+
+function {:inline} ExtendMultiset<T>(s: Multiset T, v: T): Multiset T {
+    (var len := l#Multiset(s);
+    (var cnt := v#Multiset(s)[v];
+    Multiset(v#Multiset(s)[v := (cnt + 1)], len + 1)))
+}
+
+// This function returns (s1 - s2). This function assumes that s2 is a subset of s1.
+function {:inline} SubtractMultiset<T>(s1: Multiset T, s2: Multiset T): Multiset T {
+    (var len1 := l#Multiset(s1);
+    (var len2 := l#Multiset(s2);
+    Multiset((lambda v:T :: v#Multiset(s1)[v]-v#Multiset(s2)[v]), len1-len2)))
+}
+
+function {:inline} IsEmptyMultiset<T>(s: Multiset T): bool {
+    (l#Multiset(s) == 0) &&
+    (forall v: T :: v#Multiset(s)[v] == 0)
+}
+
+function {:inline} IsSubsetMultiset<T>(s1: Multiset T, s2: Multiset T): bool {
+    (l#Multiset(s1) <= l#Multiset(s2)) &&
+    (forall v: T :: v#Multiset(s1)[v] <= v#Multiset(s2)[v])
+}
+
+function {:inline} ContainsMultiset<T>(s: Multiset T, v: T): bool {
+    v#Multiset(s)[v] > 0
+}
